solvers/8.lean
@@ -3,4 +3,4 @@ import ProjectEulerSolutions.P8
 open ProjectEulerSolutions.P8
 
 def main : IO Unit := do
-  IO.println (solve 13)
+  IO.println (solve ProjectEulerStatements.P8.bigNumber 13)
